theories/typing/int.v
@@ -330,20 +330,20 @@ Section programs.
   Lemma type_if_int it n v T1 T2:
     destruct_hint (DHintDecide (n ≠ 0)) (DestructHintIfInt n)
     (if decide (n ≠ 0) then T1 else T2) -∗
-    typed_if (IntOp it) v (n @ int it) T1 T2.
+    typed_if (IntOp it) v (v ◁ᵥ n @ int it) T1 T2.
   Proof.
     unfold destruct_hint. iIntros "Hs %Hb" => /=.
     iExists it, n. iSplit; first done. iSplit; first done.
     by do !case_decide.
   Qed.
-  Global Instance type_if_int_inst n v it : TypedIf (IntOp it) v (n @ int it) :=
+  Global Instance type_if_int_inst n v it : TypedIf (IntOp it) v (v ◁ᵥ n @ int it)%I :=
     λ T1 T2, i2p (type_if_int it n v T1 T2).
 
   Lemma type_assert_int it n s Q fn ls R v :
     (⌜n ≠ 0⌝ ∗ typed_stmt s fn ls R Q) -∗
-    typed_assert (IntOp it) v (n @ int it) s fn ls R Q.
+    typed_assert (IntOp it) v (v ◁ᵥ n @ int it) s fn ls R Q.
   Proof. iIntros "[% Hs] %Hb". iExists it, _. by iFrame. Qed.
-  Global Instance type_assert_int_inst it n v : TypedAssert (IntOp it) v (n @ int it) :=
+  Global Instance type_assert_int_inst it n v : TypedAssert (IntOp it) v (v ◁ᵥ n @ int it)%I :=
     λ s fn ls R Q, i2p (type_assert_int _ _ _ _ _ _ _ _).
 
   Inductive destruct_hint_switch_int :=
@@ -504,22 +504,22 @@ Section programs.
   Lemma type_if_bool it (b : bool) v T1 T2 :
     destruct_hint (DHintDestruct _ b) (DestructHintIfBool b)
     (if b then T1 else T2) -∗
-    typed_if (IntOp it) v (b @ boolean it) T1 T2.
+    typed_if (IntOp it) v (v ◁ᵥ b @ boolean it) T1 T2.
   Proof.
     unfold destruct_hint. iIntros "Hs %Hb".
     iExists _, _. do 2 iSplit => //. by destruct b.
   Qed.
-  Global Instance type_if_bool_inst it b v : TypedIf (IntOp it) v (b @ boolean it) :=
+  Global Instance type_if_bool_inst it b v : TypedIf (IntOp it) v (v ◁ᵥ b @ boolean it)%I :=
     λ T1 T2, i2p (type_if_bool it b v T1 T2).
 
   Lemma type_assert_bool it (b : bool) s Q fn ls R v :
     (⌜b⌝ ∗ typed_stmt s fn ls R Q) -∗
-    typed_assert (IntOp it) v (b @ boolean it) s fn ls R Q.
+    typed_assert (IntOp it) v (v ◁ᵥ b @ boolean it) s fn ls R Q.
   Proof.
     iIntros "[% Hs] %Hb". iExists it, _. iFrame "Hs".
     do 2 (iSplit; first done). by destruct b.
   Qed.
-  Global Instance type_assert_bool_inst it b v : TypedAssert (IntOp it) v (b @ boolean it) :=
+  Global Instance type_assert_bool_inst it b v : TypedAssert (IntOp it) v (v ◁ᵥ b @ boolean it)%I :=
     λ s fn ls R Q, i2p (type_assert_bool _ _ _ _ _ _ _ _).
 
   Lemma type_cast_bool b it1 it2 v T:
